systems/TreeAggregationStatic.v
@@ -908,6 +908,17 @@ Instance TreeAggregation_Aggregation_name_tot_map_bijective : MultiParamsNameTot
     tot_map_name_inverse_inv := fun _ => Logic.eq_refl
   }.
 
+Instance TreeAggregation_Aggregation_params_pt_msg_map : MultiParamsMsgPartialMap TreeAggregation_MultiParams AG.Aggregation_MultiParams :=
+  {
+    pt_map_msg := fun m => 
+      match m with 
+      | Aggregate m' => Some (AG.Aggregate m')
+      | Fail => Some AG.Fail      
+      | Level _ => None 
+      end   
+  }.
+
+
 Instance TreeAggregation_Aggregation_params_pt_ext_map : MultiParamsPartialExtendedMap TreeAggregation_MultiParams AG.Aggregation_MultiParams :=
   {
     pt_ext_map_data := fun d _ => 
@@ -923,18 +934,12 @@ Instance TreeAggregation_Aggregation_params_pt_ext_map : MultiParamsPartialExten
           end
       | AggregateRequest => (Some AG.AggregateRequest)
       | _ => None
-      end ;
-    pt_ext_map_msg := fun m => 
-      match m with 
-      | Aggregate m' => Some (AG.Aggregate m')
-      | Fail => Some AG.Fail      
-      | Level _ => None 
-      end   
+      end
   }.
 
 Lemma pt_ext_map_name_msgs_level_adjacent_empty : 
   forall fs lvo,
-  pt_ext_map_name_msgs (level_adjacent lvo fs) = [].
+  pt_map_name_msgs (level_adjacent lvo fs) = [].
 Proof.
 move => fs lvo.
 rewrite /level_adjacent NSet.fold_spec.
@@ -942,10 +947,10 @@ elim: NSet.elements => //=.
 move => n ns IH.
 rewrite {2}/level_fold /=.
 rewrite (@fold_left_level_fold_eq TreeAggregation_TreeMsg) /=.
-by rewrite pt_ext_map_name_msgs_app_distr /= -app_nil_end IH.
+by rewrite pt_map_name_msgs_app_distr /= -app_nil_end IH.
 Qed.
 
-Instance TreeAggregation_Aggregation_multi_params_pt_ext_map_congruency : MultiParamsPartialExtendedMapCongruency TreeAggregation_Aggregation_name_tot_map TreeAggregation_Aggregation_params_pt_ext_map :=
+Instance TreeAggregation_Aggregation_multi_params_pt_ext_map_congruency : MultiParamsPartialExtendedMapCongruency TreeAggregation_Aggregation_name_tot_map TreeAggregation_Aggregation_params_pt_msg_map TreeAggregation_Aggregation_params_pt_ext_map :=
   {
     pt_ext_init_handlers_eq := _ ;
     pt_ext_net_handlers_some := _ ;
@@ -1015,9 +1020,9 @@ Proof.
   * by rewrite pt_ext_map_name_msgs_level_adjacent_empty.
 Qed.
   
-Instance TreeAggregation_Aggregation_fail_msg_params_pt_ext_map_congruency : FailMsgParamsPartialExtendedMapCongruency TreeAggregation_FailMsgParams AG.Aggregation_FailMsgParams TreeAggregation_Aggregation_params_pt_ext_map := 
+Instance TreeAggregation_Aggregation_fail_msg_params_pt_ext_map_congruency : FailMsgParamsPartialMapCongruency TreeAggregation_FailMsgParams AG.Aggregation_FailMsgParams TreeAggregation_Aggregation_params_pt_msg_map := 
   {
-    pt_ext_fail_msg_fst_snd := Logic.eq_refl
+    pt_fail_msg_fst_snd := Logic.eq_refl
   }.
 
 Instance TreeAggregation_Aggregation_name_overlay_params_tot_map_congruency : NameOverlayParamsTotalMapCongruency TreeAggregation_NameOverlayParams AG.Aggregation_NameOverlayParams TreeAggregation_Aggregation_name_tot_map := 
@@ -1176,7 +1181,7 @@ Instance AggregationMsg_TreeAggregation : AggregationMsg :=
 
 Instance AggregationMsgMap_Aggregation_TreeAggregation : AggregationMsgMap AggregationMsg_TreeAggregation AG.AggregationMsg_Aggregation :=
   {
-    map_msgs := pt_ext_map_msgs ;    
+    map_msgs := pt_map_msgs ;    
   }.
 Proof.
 - elim => //=.
